theories/automation.v
@@ -1243,86 +1243,56 @@ Section instances.
     iIntros (t Ht). by iApply (big_andL_elem_of with "Hwp").
   Qed.
 
-  Lemma li_wp_read_reg r v ann es :
+  Lemma li_wpreadreg_nil r Φ:
     (find_in_context (FindRegMapsTo r) (λ rk,
       match rk with
-      | RKMapsTo v' => (⌜v = v'⌝ -∗ r ↦ᵣ v' -∗ WPasm es)
+      | RKMapsTo v' => r ↦ᵣ v' -∗ Φ v'
       | RKCol regs =>
           (tactic_hint (regcol_compute_hint (regcol_lookup (KindReg r)) regs) (λ '(_, s),
-             reg_col regs -∗ ⌜valu_has_shape v s⌝ -∗ WPasm es))
+             ∀ v', ⌜valu_has_shape v' s⌝ -∗ reg_col regs -∗ Φ v'))
       end)) -∗
-    WPasm (ReadReg r [] v ann :t: es).
+    WPreadreg r @ [] {{ Φ }}.
   Proof.
     unfold tactic_hint, regcol_compute_hint.
     iDestruct 1 as (rk) "[Hr Hwp]" => /=. case_match; simplify_eq.
-    - by iApply (wp_read_reg with "Hr").
+    - by iApply (read_reg_nil with "Hr").
     - iDestruct "Hwp" as ([??] ?%regcol_lookup_Some) "Hwp"; simplify_eq/=.
-      iDestruct (reg_col_lookup with "Hr") as (??) "[Hr Hregs]"; [done|] => /=.
-      iApply (wp_read_reg with "Hr"). iIntros (?) "Hr". subst.
-      iApply ("Hwp" with "[-] [//]"). iApply reg_col_lookup; [done|]. iExists _. by iFrame.
-  Qed.
-
-  Lemma li_wp_read_reg_struct r f v ann es :
-    (∃ vread, ⌜read_accessor [Field f] v = Some vread⌝ ∗
-     (find_in_context (FindStructRegMapsTo r f) (λ rk,
-      match rk with
-      | RKMapsTo v' => (⌜vread = v'⌝ -∗ r # f ↦ᵣ v' -∗ WPasm es)
-      | RKCol regs => tactic_hint (regcol_compute_hint (regcol_lookup_field r f) regs) (λ '(b, s),
-             ⌜valu_has_shape vread s⌝ -∗ reg_col regs -∗ WPasm es)
-      end))) -∗
-    WPasm (ReadReg r [Field f] v ann :t: es).
-  Proof.
-    unfold tactic_hint, regcol_compute_hint.
-    iDestruct 1 as (???) "[Hr Hwp]" => /=. case_match; simplify_eq.
-    - by iApply (wp_read_reg_struct with "Hr").
-    - iDestruct "Hwp" as ([b s] Hs) "Hwp"; simplify_eq/=.
-      iDestruct (regcol_lookup_field_Some with "Hr") as (???) "[Hr Hregs]"; [done|] => /=.
-      destruct b.
-      + iApply (wp_read_reg_struct with "Hr"); [done|].
-        iIntros (?) "Hr"; subst. iApply ("Hwp" with "[//]"). by iApply "Hregs".
-      + iDestruct "Hr" as "[Hr %]". iApply (wp_read_reg_acc with "Hr"); [done..|].
-        iIntros (?) "Hr"; subst. iApply ("Hwp" with "[//]"). iApply "Hregs". by iFrame.
-  Qed.
-
-  Lemma li_wp_assume_reg r v ann es :
-    (find_in_context (FindRegMapsTo r) (λ rk,
-      match rk with
-      | RKMapsTo v' => (⌜v = v'⌝ ∗ (r ↦ᵣ v' -∗ WPasm es))
-      | RKCol regs =>
-          (tactic_hint (regcol_compute_hint (regcol_lookup (KindReg r)) regs) (λ '(_, s),
-             ⌜∀ v', valu_has_shape v' s → v' = v⌝ ∗ (reg_col regs -∗ WPasm es)))
-      end)) -∗
-    WPasm (AssumeReg r [] v ann :t: es).
-  Proof.
-    unfold tactic_hint, regcol_compute_hint.
-    iDestruct 1 as (rk) "[Hr Hwp]" => /=. case_match; simplify_eq.
-    - iDestruct "Hwp" as (->) "?". by iApply (wp_assume_reg with "Hr").
-    - iDestruct "Hwp" as ([??]?%regcol_lookup_Some Hr) "Hwp"; simplify_eq/=.
       iDestruct (reg_col_lookup with "Hr") as (vact ?) "[Hr Hregs]"; [done|] => /=.
-      have ?: vact = v by naive_solver. subst.
-      iApply (wp_assume_reg with "Hr"). iIntros "Hr". iApply "Hwp".
+      iApply (read_reg_nil with "Hr").  iIntros "Hr". iApply "Hwp"; [done|].
       iApply reg_col_lookup; [done|]. iExists _. by iFrame.
   Qed.
 
-  Lemma li_wp_assume_reg_struct r f v ann es :
-    ((find_in_context (FindStructRegMapsTo r f) (λ rk,
+  Lemma li_wpreadreg_field r f Φ:
+    (find_in_context (FindStructRegMapsTo r f) (λ rk,
       match rk with
-      | RKMapsTo v' => ⌜v = v'⌝ ∗ (r # f ↦ᵣ v' -∗ WPasm es)
-      | RKCol regs => tactic_hint (regcol_compute_hint (regcol_lookup_field r f) regs) (λ '(b, s),
-          if s is ExactShape v' then ⌜v = v'⌝ ∗ (reg_col regs -∗ WPasm es) else False)
-      end))) -∗
-    WPasm (AssumeReg r [Field f] v ann :t: es).
+      | RKMapsTo v' => r # f ↦ᵣ v' -∗ Φ v'
+      | RKCol regs =>
+          (tactic_hint (regcol_compute_hint (regcol_lookup_field r f) regs) (λ '(_, s),
+             ∀ v', ⌜valu_has_shape v' s⌝ -∗ reg_col regs -∗ Φ v'))
+      end)) -∗
+    WPreadreg r @ [Field f] {{ Φ }}.
   Proof.
     unfold tactic_hint, regcol_compute_hint.
-    iDestruct 1 as (?) "[Hr Hwp]" => /=. case_match; simplify_eq.
-    - iDestruct "Hwp" as (->) "?". by iApply (wp_assume_reg_struct with "Hr").
-    - iDestruct "Hwp" as ([b []] Hs) "Hwp"; simplify_eq/= => //. iDestruct "Hwp" as (?) "Hwp". subst.
-      iDestruct (regcol_lookup_field_Some with "Hr") as (???) "[Hr Hregs]"; [done|]; simplify_eq/=.
+    iDestruct 1 as (rk) "[Hr Hwp]" => /=. case_match; simplify_eq.
+    - by iApply (read_reg_struct with "Hr").
+    - iDestruct "Hwp" as ([b s] Hs) "Hwp"; simplify_eq/=.
+      iDestruct (regcol_lookup_field_Some with "Hr") as (???) "[Hr Hregs]"; [done|] => /=.
       destruct b.
-      + iApply (wp_assume_reg_struct with "Hr"). iIntros "Hr". iApply "Hwp". by iApply "Hregs".
-      + iDestruct "Hr" as "[Hr %]". iApply (wp_assume_reg_acc with "Hr"); [done|].
-        iIntros "Hr". iApply "Hwp". iApply "Hregs". by iFrame.
+      + iApply (read_reg_struct with "Hr"). iIntros "Hr". iApply ("Hwp" with "[//]"). by iApply "Hregs".
+      + iDestruct "Hr" as "[Hr %]". iApply (read_reg_acc with "Hr"); [done..|].
+        iIntros "Hr". iApply ("Hwp" with "[//]"). iApply "Hregs". by iFrame.
   Qed.
+
+  Lemma li_wp_read_reg r v ann es al :
+    (∃ vread, ⌜read_accessor al v = Some vread⌝ ∗
+        WPreadreg r @ al {{ v', ⌜vread = v'⌝ -∗ WPasm es }}) -∗
+    WPasm (ReadReg r al v ann :t: es).
+  Proof. iDestruct 1 as (??) "Hwp". by iApply wp_read_reg. Qed.
+
+  Lemma li_wp_assume_reg r v ann es al :
+    (WPreadreg r @ al {{ v', ⌜v = v'⌝ ∗ WPasm es }}) -∗
+    WPasm (AssumeReg r al v ann :t: es).
+  Proof. apply wp_assume_reg. Qed.
 
   Lemma li_wp_write_reg r v ann es:
     (find_in_context (FindRegMapsTo r) (λ rk,
@@ -1494,47 +1464,10 @@ Section instances.
     WPexp (Val v ann) {{ Φ }}.
   Proof. apply: wpe_val. Qed.
 
-  Lemma li_wpae_var_reg r Φ ann :
-    (find_in_context (FindRegMapsTo r) (λ rk,
-      match rk with
-      | RKMapsTo v => (if v is RegVal_Base v' then r ↦ᵣ v -∗ Φ v' else False)
-      | RKCol regs =>
-          tactic_hint (regcol_compute_hint (regcol_lookup (KindReg r)) regs) (λ '(_, s),
-           ∀ v, ⌜valu_has_shape v s⌝ -∗ ∃ v', ⌜v = RegVal_Base v'⌝ ∗ (reg_col regs -∗ Φ v')
-             )
-      end)) -∗
-    WPaexp (AExp_Val (AVal_Var r []) ann) {{ Φ }}.
-  Proof.
-    unfold tactic_hint, regcol_compute_hint.
-    iDestruct 1 as (rk) "[Hr Hwp]" => /=. case_match; simplify_eq.
-    - case_match => //; subst. by iApply (wpae_var_reg with "Hr").
-    - iDestruct "Hwp" as ([??] ?%regcol_lookup_Some) "Hwp"; simplify_eq/=.
-      iDestruct (reg_col_lookup with "Hr") as (??) "[Hr Hregs]"; [done|] => /=.
-      iDestruct ("Hwp" with "[//]") as (? ->) "Hwp".
-      iApply (wpae_var_reg with "Hr"). iIntros "Hr". iApply "Hwp".
-      iApply reg_col_lookup; [done|]. iExists _. by iFrame.
-  Qed.
-
-  Lemma li_wpae_var_struct r f Φ ann :
-    (find_in_context (FindStructRegMapsTo r f) (λ rk,
-      match rk with
-      | RKMapsTo v => (if v is RegVal_Base v' then r # f ↦ᵣ v -∗ Φ v' else False)
-      | RKCol regs => tactic_hint (regcol_compute_hint (regcol_lookup_field r f) regs) (λ '(b, s),
-           ∀ v, ⌜valu_has_shape v s⌝ -∗ if v is RegVal_Base v' then (reg_col regs -∗ Φ v') else False)
-      end)) -∗
-    WPaexp (AExp_Val (AVal_Var r [Field f]) ann) {{ Φ }}.
-  Proof.
-    unfold tactic_hint, regcol_compute_hint.
-    iDestruct 1 as (rk) "[Hr Hwp]" => /=. case_match; simplify_eq.
-    - case_match => //; subst. by iApply (wpae_var_struct with "Hr").
-    - iDestruct "Hwp" as ([b s] Hs) "Hwp"; simplify_eq/=.
-      iDestruct (regcol_lookup_field_Some with "Hr") as (???) "[Hr Hregs]"; [done|]; simplify_eq/=.
-      iDestruct ("Hwp" with "[//]") as "Hwp". destruct v => //.
-      destruct b.
-      + iApply (wpae_var_struct with "Hr"). iIntros "Hr". iApply "Hwp". by iApply "Hregs".
-      + iDestruct "Hr" as "[Hr %]". iApply (wpae_var_reg_acc with "Hr"); [done|].
-        iIntros "Hr". iApply "Hwp". iApply "Hregs". by iFrame.
-  Qed.
+  Lemma li_wpae_var_reg r al Φ ann :
+    WPreadreg r @ al {{ v', if v' is RegVal_Base v'' then Φ v'' else False }} -∗
+    WPaexp (AExp_Val (AVal_Var r al) ann) {{ Φ }}.
+  Proof. apply wpae_var_reg. Qed.
 
   Lemma li_wpae_bits b Φ ann:
     Φ (Val_Bits b) -∗
@@ -1719,10 +1652,8 @@ Ltac liAAsm :=
     | tcases _ => notypeclasses refine (tac_fast_apply (li_wp_cases _) _)
     | ?e :t: _ =>
       lazymatch e with
-      | ReadReg _ [] _ _ => notypeclasses refine (tac_fast_apply (li_wp_read_reg _ _ _ _) _)
-      | ReadReg _ [Field _] _ _ => notypeclasses refine (tac_fast_apply (li_wp_read_reg_struct _ _ _ _ _) _)
-      | AssumeReg _ [] _ _ => notypeclasses refine (tac_fast_apply (li_wp_assume_reg _ _ _ _) _)
-      | AssumeReg _ [Field _] _ _ => notypeclasses refine (tac_fast_apply (li_wp_assume_reg_struct _ _ _ _ _) _)
+      | ReadReg _ _ _ _ => notypeclasses refine (tac_fast_apply (li_wp_read_reg _ _ _ _ _) _)
+      | AssumeReg _ _ _ _ => notypeclasses refine (tac_fast_apply (li_wp_assume_reg _ _ _ _ _) _)
       | WriteReg _ [] _ _ => notypeclasses refine (tac_fast_apply (li_wp_write_reg _ _ _ _) _)
       | WriteReg _ [Field _] _ _ => notypeclasses refine (tac_fast_apply (li_wp_write_reg_struct _ _ _ _ _) _)
       | BranchAddress _ _ => notypeclasses refine (tac_fast_apply (li_wp_branch_address _ _ _) _)
@@ -1745,6 +1676,10 @@ Ltac liAAsm :=
     end
   | |- envs_entails ?Δ (instr_pre' _ _ _) =>
     notypeclasses refine (tac_fast_apply (li_instr_pre _ _ _) _)
+  | |- envs_entails ?Δ (wpreadreg _ [] _) =>
+     notypeclasses refine (tac_fast_apply (li_wpreadreg_nil _ _) _)
+  | |- envs_entails ?Δ (wpreadreg _ [Field _] _) =>
+     notypeclasses refine (tac_fast_apply (li_wpreadreg_field _ _ _) _)
   end.
 
 Ltac liAExp :=
@@ -1761,8 +1696,7 @@ Ltac liAExp :=
     (* end *)
   | |- envs_entails ?Δ (wp_a_exp ?e _) =>
     lazymatch e with
-    | AExp_Val (AVal_Var _ []) _ => notypeclasses refine (tac_fast_apply (li_wpae_var_reg _ _ _) _)
-    | AExp_Val (AVal_Var _ [Field _]) _ => notypeclasses refine (tac_fast_apply (li_wpae_var_struct _ _ _ _) _)
+    | AExp_Val (AVal_Var _ _) _ => notypeclasses refine (tac_fast_apply (li_wpae_var_reg _ _ _ _) _)
     | AExp_Val (AVal_Bits _) _ => notypeclasses refine (tac_fast_apply (li_wpae_bits _ _ _) _)
     | AExp_Val (AVal_Bool _) _ => notypeclasses refine (tac_fast_apply (li_wpae_bool _ _ _) _)
     | AExp_Val (AVal_Enum _) _ => notypeclasses refine (tac_fast_apply (li_wpae_enum _ _ _) _)
